@prefix : <http://www.semanticweb.org/asset#> .
@prefix fso: <http://www.semanticweb.org/functional-system-ontology/> .
@prefix lis: <http://standards.iso.org/iso/15926/part14/> .
@prefix owl: <http://www.w3.org/2002/07/owl#> .
@prefix rdf: <http://www.w3.org/1999/02/22-rdf-syntax-ns#> .
@prefix xml: <http://www.w3.org/XML/1998/namespace> .
@prefix xsd: <http://www.w3.org/2001/XMLSchema#> .
@prefix fmea: <http://www.semanticweb.org/fmea-iso/> .
@prefix rdfs: <http://www.w3.org/2000/01/rdf-schema#> .
@prefix asset: <http://www.semanticweb.org/asset/> .
@base <http://www.semanticweb.org/asset> .

<http://www.semanticweb.org/asset> rdf:type owl:Ontology ;
                                    owl:imports <http://www.semanticweb.org/fmea-iso> .

#################################################################
#    Classes
#################################################################

###  http://www.semanticweb.org/asset/Chamber
asset:Chamber rdf:type owl:Class ;
              rdfs:subClassOf fso:Component ;
              rdfs:label "Chamber" .


###  http://www.semanticweb.org/asset/CollectionChamber
asset:CollectionChamber rdf:type owl:Class ;
                        rdfs:subClassOf asset:Chamber ;
                        rdfs:label "Collection chamber" .


###  http://www.semanticweb.org/asset/CondensateSystem
asset:CondensateSystem rdf:type owl:Class ;
                       rdfs:subClassOf lis:System ;
                       rdfs:label "Condensate System" .


###  http://www.semanticweb.org/asset/CoolingDoor
asset:CoolingDoor rdf:type owl:Class ;
                  rdfs:subClassOf fso:Component ;
                  rdfs:label "Cooling door" .


###  http://www.semanticweb.org/asset/DrainPipe
asset:DrainPipe rdf:type owl:Class ;
                rdfs:subClassOf fso:Component ;
                rdfs:label "Drain pipe" .


###  http://www.semanticweb.org/asset/EmergencyDoorsSystem
asset:EmergencyDoorsSystem rdf:type owl:Class ;
                           rdfs:subClassOf lis:System ;
                           rdfs:label "Emergency Doors System" .


###  http://www.semanticweb.org/asset/FailureDueToEarthFault
asset:FailureDueToEarthFault rdf:type owl:Class ;
                             rdfs:subClassOf fmea:FailureEvent .


###  http://www.semanticweb.org/asset/FailureDueToOvercurrent
asset:FailureDueToOvercurrent rdf:type owl:Class ;
                              rdfs:subClassOf fmea:FailureEvent .


###  http://www.semanticweb.org/asset/FailureDueToShortCircuit
asset:FailureDueToShortCircuit rdf:type owl:Class ;
                               rdfs:subClassOf fmea:FailureEvent .


###  http://www.semanticweb.org/asset/Fan
asset:Fan rdf:type owl:Class ;
          rdfs:subClassOf fso:Component ;
          rdfs:label "Fan" .


###  http://www.semanticweb.org/asset/Filter
asset:Filter rdf:type owl:Class ;
             rdfs:subClassOf fso:Component ;
             rdfs:label "Filter " .


###  http://www.semanticweb.org/asset/HeatExchanger
asset:HeatExchanger rdf:type owl:Class ;
                    rdfs:subClassOf fso:Component ;
                    rdfs:label "Heat exchanger" .


###  http://www.semanticweb.org/asset/Heater
asset:Heater rdf:type owl:Class ;
             rdfs:subClassOf fso:Component ;
             rdfs:label "Heater" .


###  http://www.semanticweb.org/asset/HeaterSystem
asset:HeaterSystem rdf:type owl:Class ;
                   rdfs:subClassOf lis:System ;
                   rdfs:label "Heater System" .


###  http://www.semanticweb.org/asset/HeatingAttemptAndNoHeat
asset:HeatingAttemptAndNoHeat rdf:type owl:Class ;
                              rdfs:subClassOf asset:HeatingProcess ,
                                              fmea:FailureEffect ;
                              rdfs:label "Heating attempt and no heat" .


###  http://www.semanticweb.org/asset/HeatingAttemptAndPartialHeat
asset:HeatingAttemptAndPartialHeat rdf:type owl:Class ;
                                   rdfs:subClassOf asset:HeatingProcess ,
                                                   fmea:FailureEffect ;
                                   rdfs:label "Heating attempt and partial heat" .


###  http://www.semanticweb.org/asset/HeatingProcess
asset:HeatingProcess rdf:type owl:Class ;
                     rdfs:subClassOf fso:Process ;
                     rdfs:label "Heating Process" .


###  http://www.semanticweb.org/asset/LeakageSystem
asset:LeakageSystem rdf:type owl:Class ;
                    rdfs:subClassOf lis:System ;
                    rdfs:label "Leakage System" .


###  http://www.semanticweb.org/asset/ObservationOfEarthFault
asset:ObservationOfEarthFault rdf:type owl:Class ;
                              rdfs:subClassOf fmea:FailureModeObservation ;
                              rdfs:comment "'Observation of earth fault' is a subclass of 'FailureModeObservation'. It refers to the 'Failure Mode' column in Table 2." .


###  http://www.semanticweb.org/asset/ObservationOfOvercurrent
asset:ObservationOfOvercurrent rdf:type owl:Class ;
                               rdfs:subClassOf fmea:FailureModeObservation ;
                               rdfs:comment "'Observation of over current' is a subclass of 'FailureModeObservation'. It refers to the 'Failure Mode' column in Table 2." .


###  http://www.semanticweb.org/asset/ObservationOfShortCircuit
asset:ObservationOfShortCircuit rdf:type owl:Class ;
                                rdfs:subClassOf fmea:FailureModeObservation ;
                                rdfs:comment "'Observation of short circuit' is a subclass of 'FailureModeObservation'. It refers to the 'Failure Mode' column in Table 2." .


###  http://www.semanticweb.org/asset/Sump
asset:Sump rdf:type owl:Class ;
           rdfs:subClassOf fso:Component ;
           rdfs:label "Sump" .


###  http://www.semanticweb.org/asset/TerminalBoxCables
asset:TerminalBoxCables rdf:type owl:Class ;
                        rdfs:subClassOf fso:Component ;
                        rdfs:label "Terminal box & cables" .


###  http://www.semanticweb.org/asset/VentilationSystem
asset:VentilationSystem rdf:type owl:Class ;
                        rdfs:subClassOf lis:System ;
                        rdfs:label "Ventilation System" .


###  http://www.semanticweb.org/fmea-iso/FailureEffect
fmea:FailureEffect <http://www.w3.org/2004/02/skos/core#definition> "The consequence of a `FailureMode' in terms of the \\newline operation, function or status of the item (IEC 60812:2008)." ;
                   <http://www.w3.org/2004/02/skos/core#note> "An FSO: process that results from an FMO: functional failure." .


###  http://www.semanticweb.org/fmea-iso/FailureEvent
fmea:FailureEvent <http://www.w3.org/2004/02/skos/core#definition> "A process or  activity which results in functional failure of an item. Equivalent to (hasParticipant some Component) and (resultsIn some FunctionalFailure)." ;
                  <http://www.w3.org/2004/02/skos/core#note> "An FSO: process that results in an FMO: functional failure" .


###  http://www.semanticweb.org/fmea-iso/FailureModeObservation
fmea:FailureModeObservation <http://www.w3.org/2004/02/skos/core#definition> "The effect by which a failure is observed on the failed item (ISO 14224:2006)" ;
                            <http://www.w3.org/2004/02/skos/core#note> "An ISO: information object that represents an FMO: functional failure." .


###  http://www.semanticweb.org/fmea-iso/FinalFailureEffect
fmea:FinalFailureEffect <http://www.w3.org/2004/02/skos/core#definition> "The final consequence on the system (IEC 60812:2008)" ;
                        <http://www.w3.org/2004/02/skos/core#note> "The terminal FSO: process from the set of FSO: processes that result from an FMO: functional failure." .


###  http://www.semanticweb.org/fmea-iso/FunctionalFailure
fmea:FunctionalFailure <http://www.w3.org/2004/02/skos/core#definition> "The termination of ability of an item to perform a required function (IEC 60812:2008). Equivalent to (representedBy some FailureModeObservation) and \\newline (resultsIn some FailureEffect)." ;
                       <http://www.w3.org/2004/02/skos/core#note> "FSO: process which is the result of an FMO: failure event and results in an FMO: failure effect. It is represented by some FMO: failure mode observation." .


###  http://www.semanticweb.org/fmea-iso/Malfunction
fmea:Malfunction <http://www.w3.org/2004/02/skos/core#definition> "The disposition of an item to fail to perform a required function." ;
                 <http://www.w3.org/2004/02/skos/core#note> "An ISO: disposition that is only realized in an FMO: failure event." .


#################################################################
#    Individuals
#################################################################

###  http://www.semanticweb.org/asset/air_water_heat_exchanger
asset:air_water_heat_exchanger rdf:type owl:NamedIndividual ,
                                        asset:HeatExchanger ;
                               rdfs:comment "'Air / water heat exchanger' is an individual from Class 'Heat exchanger'. It is represented as element 20.2.2 in Figure 1. It is a subsystem to the ‘Ventilation and cooling system'" ;
                               rdfs:label "Air / water heat exchanger" .


###  http://www.semanticweb.org/asset/condensate_drain_pipe
asset:condensate_drain_pipe rdf:type owl:NamedIndividual ,
                                     asset:DrainPipe ;
                            rdfs:comment "'Condensate drain pipes (small bore)' is an individual from Class 'Drain pipe'. It is represented as element 20.4.1 in Figure 1. It is a subsystem to the ‘Condensate / cooling-water drain system'" ;
                            rdfs:label "Condensate drain pipes (small bore)" .


###  http://www.semanticweb.org/asset/condensate_drain_system
asset:condensate_drain_system rdf:type owl:NamedIndividual ,
                                       asset:CondensateSystem ;
                              lis:hasFunctionalPart asset:condensate_drain_pipe ,
                                                    asset:leak_detection_chamber ,
                                                    asset:leakage_collection_area ,
                                                    asset:leakage_drain_pipe ,
                                                    asset:leakage_drain_pipe_from_leak_detect_chamber ,
                                                    asset:sump ;
                              rdfs:comment "'Condensate / cooling-water drain system' is an individual from Class 'Condensate system'. It is represented as element 20.4 in Figure 1. It is a subsystem to the ‘Enclosure heating, ventilation and cooling system'" ;
                              rdfs:label "Condensate / cooling-water drain system" .


###  http://www.semanticweb.org/asset/emergency_cooling_doors
asset:emergency_cooling_doors rdf:type owl:NamedIndividual ,
                                       asset:CoolingDoor ;
                              rdfs:comment "'Emergency cooling (inlet / outlet) doors' is an individual from Class 'Cooling door'. It is represented as element 20.3 in Figure 1. It is a subsystem to the ‘Enclosure heating, ventilation and cooling system'" ;
                              rdfs:label "Emergency cooling (inlet / outlet) doors" .


###  http://www.semanticweb.org/asset/enclosure_heating_ventilation_and_cooling_system
asset:enclosure_heating_ventilation_and_cooling_system rdf:type owl:NamedIndividual ,
                                                                fso:AncillarySystem ;
                                                       lis:hasFunctionalPart asset:condensate_drain_system ,
                                                                             asset:emergency_cooling_doors ,
                                                                             asset:heater_system ,
                                                                             asset:ventilation_and_cooling_system ;
                                                       rdfs:comment "'Enclosure heating, ventilation and cooling system' is an individual from Class 'AncillarySystem'. It is represented as element 20 in Figure 1." ;
                                                       rdfs:label "Enclosure heating, ventilation and cooling system" .


###  http://www.semanticweb.org/asset/failure_effect_of_loss_of_all_heating
asset:failure_effect_of_loss_of_all_heating rdf:type owl:NamedIndividual ,
                                                     asset:HeatingAttemptAndPartialHeat ,
                                                     fmea:FailureEffect ;
                                            rdfs:comment "'Failure effect loss of all heating' is an individual of class 'Failure effect'. It refers to the 'Failure Effect' column in Table 2." ;
                                            rdfs:label "Failure effect loss of all heating" ;
                                            rdfs:seeAlso "Initial Failure Effect"^^xsd:string .


###  http://www.semanticweb.org/asset/failure_effect_of_reduced_heating
asset:failure_effect_of_reduced_heating rdf:type owl:NamedIndividual ,
                                                 asset:HeatingAttemptAndPartialHeat ,
                                                 fmea:FailureEffect ;
                                        rdfs:comment "'Failure effect of reduced heating' is an individual of class 'Failure effect'. It refers to the 'Failure Effect' column in Table 2." ;
                                        rdfs:label "Failure effect of reduced heating" ;
                                        rdfs:seeAlso "Initial Failure Effect"^^xsd:string .


###  http://www.semanticweb.org/asset/failure_event_due_to_heaters_overcurrent
asset:failure_event_due_to_heaters_overcurrent rdf:type owl:NamedIndividual ,
                                                        asset:FailureDueToOvercurrent ;
                                               lis:hasParticipant asset:heaters ;
                                               fmea:resultsIn asset:functional_failure_of_not_heating_enclosure ;
                                               rdfs:comment "'heaters overcurrent failure event' is an individual of class 'FailureDueToOvercurrent'." ;
                                               rdfs:label "heaters overcurrent failure event" .


###  http://www.semanticweb.org/asset/fans_and_fan_hubs
asset:fans_and_fan_hubs rdf:type owl:NamedIndividual ,
                                 asset:VentilationSystem ;
                        rdfs:comment "'Fans and fan hubs' is an individual from Class 'Ventilation system'. It is represented as element 20.2.1 in Figure 1. It is a subsystem to the ‘Ventilation and cooling system'" ;
                        rdfs:label "Fans and fan hubs" .


###  http://www.semanticweb.org/asset/final_failure_effect
asset:final_failure_effect rdf:type owl:NamedIndividual ,
                                    asset:HeatingAttemptAndPartialHeat ,
                                    fmea:FinalFailureEffect ;
                           rdfs:comment "Reduced heating"^^xsd:string ;
                           rdfs:seeAlso "Final Failure Effect"^^xsd:string .


###  http://www.semanticweb.org/asset/functional_failure_of_not_heating_enclosure
asset:functional_failure_of_not_heating_enclosure rdf:type owl:NamedIndividual ,
                                                           fmea:FunctionalFailure ;
                                                  lis:representedBy asset:observation_of_over_current_due_to_burnt_out_heater ;
                                                  fmea:resultsIn asset:failure_effect_of_reduced_heating ;
                                                  rdfs:comment "'Functional failure of not heating enclosure' is an individual of class 'FunctionalFailure'." ;
                                                  rdfs:label "Functional failure of not heating enclosure" .


###  http://www.semanticweb.org/asset/heater_system
asset:heater_system rdf:type owl:NamedIndividual ,
                             asset:HeaterSystem ;
                    lis:hasFunctionalPart asset:heaters ;
                    rdfs:comment "'Heater system' is an individual from Class 'Heater system'. It is represented as element 20.1 in Figure 1. It is a subsystem to the ‘Enclosure heating, ventilation and cooling system'" ;
                    rdfs:label "Heater system" .


###  http://www.semanticweb.org/asset/heater_terminal_box
asset:heater_terminal_box rdf:type owl:NamedIndividual ,
                                   asset:TerminalBoxCables ;
                          rdfs:comment "'Heater terminal box, terminals / cables' is an individual from Class 'Terminal box cables'. It is represented as element 20.1.2 in Figure 1. It is a subsystem to the ‘Heater System'" ;
                          rdfs:label "Heater terminal box, terminals / cables" .


###  http://www.semanticweb.org/asset/heaters
asset:heaters rdf:type owl:NamedIndividual ,
                       asset:Heater ;
              fmea:hasMalfunction asset:malfunction_due_to_earth_fault ,
                                  asset:malfunction_due_to_over_current ,
                                  asset:malfunction_due_to_short_circuit ;
              rdfs:comment "'heaters' is an individual from Class 'Heater'. It is represented as element in Figure 1. It is a subsystem to the ‘Heater System'" ;
              rdfs:label "heaters" .


###  http://www.semanticweb.org/asset/heating_function
asset:heating_function rdf:type owl:NamedIndividual ,
                                lis:Function ;
                       lis:realizedIn asset:heating_process ;
                       rdfs:comment "'Heating function' is an individual of class 'Function'. It refers to the 'Function' column in Table 2." ,
                                    "To heat up enclosure" ;
                       rdfs:label "Heating function" .


###  http://www.semanticweb.org/asset/heating_process
asset:heating_process rdf:type owl:NamedIndividual ,
                               asset:HeatingProcess ;
                      lis:hasParticipant asset:heaters ;
                      rdfs:comment "'Heating process' is an individual of class 'HeatingProcess'." ;
                      rdfs:label "Heating process" .


###  http://www.semanticweb.org/asset/leak_detection_chamber
asset:leak_detection_chamber rdf:type owl:NamedIndividual ,
                                      asset:Chamber ;
                             rdfs:comment "'Leak detection chamber' is an individual from Class 'Chamber'. It is represented as element 20.4.5 in Figure 1. It is a subsystem to the ‘Condensate / cooling-water drain system'" ;
                             rdfs:label "Leak detection chamber" .


###  http://www.semanticweb.org/asset/leakage_collection_area
asset:leakage_collection_area rdf:type owl:NamedIndividual ,
                                       asset:CollectionChamber ;
                              rdfs:comment "'Leakage collection area' is an individual from Class 'Collection Chamber'. It is represented as element 20.4.6 in Figure 1. It is a subsystem to the ‘Condensate / cooling-water drain system'" ;
                              rdfs:label "Leakage collection area" .


###  http://www.semanticweb.org/asset/leakage_drain_pipe
asset:leakage_drain_pipe rdf:type owl:NamedIndividual ,
                                  asset:DrainPipe ;
                         rdfs:comment "'Condensate / leakage drain pipes' is an individual from Class 'Drain pipe'. It is represented as element 20.4.2 in Figure 1. It is a subsystem to the ‘Condensate / cooling-water drain system'" ;
                         rdfs:label "Condensate / leakage drain pipes" .


###  http://www.semanticweb.org/asset/leakage_drain_pipe_from_leak_detect_chamber
asset:leakage_drain_pipe_from_leak_detect_chamber rdf:type owl:NamedIndividual ,
                                                           asset:DrainPipe ;
                                                  rdfs:comment "'Leakage drain pipe from leak detect chamber' is an individual from Class 'Drain pipe'. It is represented as element 20.4.3 in Figure 1. It is a subsystem to the ‘Condensate / cooling-water drain system'" ;
                                                  rdfs:label "Leakage drain pipe from leak detect chamber" .


###  http://www.semanticweb.org/asset/malfunction_due_to_earth_fault
asset:malfunction_due_to_earth_fault rdf:type owl:NamedIndividual ,
                                              fmea:Malfunction ;
                                     rdfs:comment "'Malfuction due to earth fault' is an individual of class 'Malfunction'." ,
                                                  "The disposition to not heat up the enclosure" ;
                                     rdfs:label "heaters malfunction due to earth fault" .


###  http://www.semanticweb.org/asset/malfunction_due_to_over_current
asset:malfunction_due_to_over_current rdf:type owl:NamedIndividual ,
                                               fmea:Malfunction ;
                                      lis:realizedIn asset:failure_event_due_to_heaters_overcurrent ;
                                      rdfs:comment "'Malfuction due to over current' is an individual of class 'Malfunction'." ,
                                                   "A disposition to only partially heat up the enclosure" ;
                                      rdfs:label "heaters malfunction due to over current" .


###  http://www.semanticweb.org/asset/malfunction_due_to_short_circuit
asset:malfunction_due_to_short_circuit rdf:type owl:NamedIndividual ,
                                                fmea:Malfunction ;
                                       rdfs:comment "'Malfuction due to short circuit' is an individual of class 'Malfunction'." ,
                                                    "The disposition to not heat up the enclosure" ;
                                       rdfs:label "heaters malfunction due to short circuit" .


###  http://www.semanticweb.org/asset/observation_of_over_current_due_to_burnt_out_heater
asset:observation_of_over_current_due_to_burnt_out_heater rdf:type owl:NamedIndividual ,
                                                                   asset:ObservationOfOvercurrent ;
                                                          rdfs:comment "'Observation of over current due to burnt out heater' is an individual of class 'Failure mode observation'. It refers to the 'Failure Mode' column in Table 2." ;
                                                          rdfs:label "Observation of over current due to burnt out heater" .


###  http://www.semanticweb.org/asset/plastic_foam_air_filters
asset:plastic_foam_air_filters rdf:type owl:NamedIndividual ,
                                        asset:Filter ;
                               rdfs:comment "'Plastic foam air filters' is an individual from Class 'Filter'. It is represented as element 20.2.3 in Figure 1. It is a subsystem to the ‘Ventilation and cooling system'" ;
                               rdfs:label "Plastic foam air filters" .


###  http://www.semanticweb.org/asset/sump
asset:sump rdf:type owl:NamedIndividual ,
                    asset:Sump ;
           rdfs:comment "'sump' is an individual from Class 'Sump'. It is represented as element 20.4.4 in Figure 1. It is a subsystem to the ‘Condensate / cooling-water drain system'" ;
           rdfs:label "sump" .


###  http://www.semanticweb.org/asset/ventilation_and_cooling_system
asset:ventilation_and_cooling_system rdf:type owl:NamedIndividual ,
                                              asset:VentilationSystem ;
                                     lis:hasFunctionalPart asset:air_water_heat_exchanger ,
                                                           asset:fans_and_fan_hubs ,
                                                           asset:plastic_foam_air_filters ;
                                     rdfs:comment "'Ventilation and cooling system' is an individual from Class 'Ventilation system'. It is represented as element 20.2 in Figure 1. It is a subsystem to the ‘Enclosure heating, ventilation and cooling system'" ;
                                     rdfs:label "Ventilation and cooling system" .


#################################################################
#    Annotations
#################################################################

fmea:ObjectInFaultState <http://www.w3.org/2004/02/skos/core#note> "An ISO: functional object that has some realized FMO: malfunction" ;
                        <http://www.w3.org/2004/02/skos/core#definition> "The state of an item resulting from a `Malfunction'" .


###  Generated by the OWL API (version 4.5.9.2019-02-01T07:24:44Z) https://github.com/owlcs/owlapi
